more progress manually applying monotonicity invariants to paxos. Implement custom monotonic types MonotonicVBOption and MonotonicReceivedAccepts

messageInvariantPrototypes/paxos/types.dfy
@@ -9,18 +9,6 @@ type LearnerId = nat
 type Value(!new)
 datatype ValBal = VB(v:Value, b:LeaderId)
 
-datatype MonotonicVBOption = MVBSome(value: ValBal) | MVBNone
-{
-  ghost predicate SatisfiesMonotonic(past: MonotonicVBOption) {
-    past.MVBSome? ==> (this.MVBSome? && past.value.b <= this.value.b)
-  }
-
-  ghost function ToOption() : Option<ValBal> {
-    if this.MVBNone? then None
-    else Some(this.value)
-  }
-}
-
 datatype Message = Prepare(bal:LeaderId)
                 | Promise(bal:LeaderId, acc:AcceptorId, vbOpt:Option<ValBal>)  //valbal is the value-ballot pair with which the value was accepted
                 | Propose(bal:LeaderId, val:Value)
@@ -36,17 +24,31 @@ datatype Message = Prepare(bal:LeaderId)
 
 datatype MessageOps = MessageOps(recv:Option<Message>, send:Option<Message>)
 
-// Lemma: Given b1 < b2, there is a finite, strictly ordered sequence 
-// [b1, b_a, b_b, ... , b_2] such that for all ballots b where b1 < b < b2, b in seq
-lemma FiniteBallots(b1: LeaderId, b2: LeaderId) returns (res: seq<LeaderId>)
-  requires b1 < b2
-  ensures SeqIsComplete(res, b1, b2)
+
+
+/// Some custom monotonic datatypes
+
+datatype MonotonicVBOption = MVBSome(value: ValBal) | MVBNone
 {
-  if b1 == b2 - 1 {
-    return [b1, b2];
-  } else {
-    var sub := FiniteBallots(b1, b2-1);
-    return sub + [b2];
+  ghost predicate SatisfiesMonotonic(past: MonotonicVBOption) {
+    past.MVBSome? ==> (this.MVBSome? && past.value.b <= this.value.b)
+  }
+
+  ghost function ToOption() : Option<ValBal> {
+    if this.MVBNone? then None
+    else Some(this.value)
+  }
+}
+
+datatype MonotonicReceivedAccepts = RA(m: map<ValBal, set<AcceptorId>>) 
+{
+  ghost predicate SatisfiesMonotonic(past: MonotonicReceivedAccepts) {
+    forall vb | 
+    && vb in past.m 
+    :: 
+      && 0 < |past.m[vb]|
+      && vb in this.m
+      && past.m[vb] <= this.m[vb]
   }
 }
 }
